continue cleanup

Computability/Basic.lean
@@ -1,123 +1,476 @@
-import Computability.Oracle
-import Mathlib.Order.Antisymmetrization
+import Computability.Label
+-- import Computability.Basic
+import Computability.Encoding
+import Mathlib.Data.PFun
+import Mathlib.Data.Nat.Dist
 
-@[simp] abbrev TuringReducible (f g : ℕ → ℕ) : Prop := Nat.RecursiveIn g f
-@[simp] abbrev TuringReducibleStrict (f g : ℕ → ℕ) : Prop := Nat.RecursiveIn g f ∧ ¬ Nat.RecursiveIn f g
-@[simp] abbrev TuringEquivalent (f g : ℕ → ℕ) : Prop := AntisymmRel TuringReducible f g
+open Classical
+open Computability.Code
+open Nat
 
-@[reducible,simp,inherit_doc] scoped[Computability] infix:50 " ≤ᵀᶠ " => TuringReducible
-@[reducible,simp,inherit_doc] scoped[Computability] infix:50 " ≡ᵀᶠ " => TuringEquivalent
-@[reducible,simp,inherit_doc] scoped[Computability] infix:50 " <ᵀᶠ " => TuringReducibleStrict
 
-open scoped Computability
+-- general helper functions
+theorem pair_nonzero_right_pos_aux : ¬ (Nat.pair x (s+1)=0) := by
+  rw  [show 0=Nat.pair 0 0 from rfl]
+  rw [pair_eq_pair]
+  intro h
+  have hr := h.right
+  contradiction
+@[simp] theorem pair_nonzero_right_pos : (Nat.pair x (s+1))>0 := by
+  exact zero_lt_of_ne_zero pair_nonzero_right_pos_aux
+@[simp] theorem map_getI : (List.map (f) (List.range (s + 1))).getI x = if x<s+1 then f x else 0 := by
+  unfold List.getI
+  cases Classical.em (x<s+1) with
+  | inl h => simp [h]
+  | inr h => simp [h]
+theorem pair_r_gt0 {x} : x>0→(Nat.pair y x)>0 := by
+  contrapose
+  simp
+  intro h
+  rw [show x=(Nat.pair y x).unpair.2 from by simp [unpair_pair]]
+  rw [h]
+  simp [unpair_zero]
+theorem pair_l_gt0 {x} : x>0→(Nat.pair x y)>0 := by
+  contrapose
+  simp
+  intro h
+  rw [show x=(Nat.pair x y).unpair.1 from by simp [unpair_pair]]
+  rw [h]
+  simp [unpair_zero]
+-- general lemmas for later theorems
+protected theorem isSome.bind {o : Option α} (h : o.isSome) (f : α → Option β) : o.bind f = f (o.get h) := by
+  have : o = some (o.get h) := by exact Option.eq_some_of_isSome h
+  ext b
+  constructor
+  intro h2
+  rw [this] at h2
+  simp only [Option.bind_some] at h2
+  exact h2
 
-protected theorem TuringReducible.refl (f : ℕ → ℕ) : f ≤ᵀᶠ f := by exact Nat.RecursiveIn.oracle
-protected theorem TuringReducible.rfl : f ≤ᵀᶠ f := .refl _
+  intro h2
+  rw [this]
+  simp only [Option.bind_some]
+  exact h2
+theorem listrwgen (n): (List.range (n + 1)).reverse = n :: (List.range n).reverse := by
+  simp
+  exact List.range_succ
+theorem ne_of_mem_imp_not_mem {y:Part ℕ} (h:x∈y) (h2:x≠z) : z∉y := by
+  have aux: y=Part.some x := by exact Part.eq_some_iff.mpr h
+  rw [aux]
+  aesop? says
+    subst aux
+    simp_all only [ne_eq, Part.mem_some_iff]
+    apply Aesop.BuiltinRules.not_intro
+    intro a
+    subst a
+    simp_all only [not_true_eq_false]
+theorem opt_ne_of_mem_imp_not_mem {y:Option ℕ} (h:x∈y) (h2:x≠z) : z∉y := by
+  aesop
+lemma forall_mem_part {y:Part ℕ} (h1:y.Dom) (h2:∀ x ∈ y, x = c) : c∈y := by
+  contrapose h2
+  simp
+  use y.get h1
+  constructor
+  exact Part.get_mem h1
+  apply Aesop.BuiltinRules.not_intro
+  intro a
+  subst a
+  have : y.get h1 ∈ y := by exact Part.get_mem h1
+  contradiction
+lemma forall_mem_option {y:Option ℕ} (h1:y.isSome) (h2:∀ x ∈ y, x = c) : c∈y := by
+  contrapose h2
+  simp
+  use y.get h1
+  constructor
+  exact Option.eq_some_of_isSome h1
+  apply Aesop.BuiltinRules.not_intro
+  intro a
+  subst a
+  have : y.get h1 ∈ y := by exact Option.eq_some_of_isSome h1
+  contradiction
+-- helper functions for Part/Option
+theorem Part.eq_some_imp_dom {p:Part ℕ} : p=Part.some x → p.Dom := by
+  intro a
+  subst a
+  exact trivial
+theorem Part.mem_imp_dom {p:Part ℕ} : x∈p → p.Dom := λ h ↦ Part.eq_some_imp_dom (Part.eq_some_iff.mpr h)
+theorem Part.dom_imp_some {x:Part ℕ} (h:x.Dom) : x=Part.some (x.get h) := by
+  exact Part.get_eq_iff_eq_some.mp rfl
+theorem Option.dom_imp_some {x:Option ℕ} (h:x.isSome) : x=some (x.get h) := by
+  exact Option.eq_some_of_isSome h
+theorem Option.isSome_iff_mem {o:Option β}: o.isSome ↔ (∃z,z∈o) := by
+  have h1 := @Option.isSome_iff_exists β o
+  simp [h1]
+lemma isSome_iff_not_none : (¬o=Option.none)↔(o.isSome) := by
+  apply Iff.intro
+  · intro a
+    simp [Option.eq_none_iff_forall_ne_some] at a
+    rcases a with ⟨h1,h2⟩
+    exact Option.isSome_of_mem h2
+  · intro a
+    apply Aesop.BuiltinRules.not_intro
+    intro a_1
+    subst a_1
+    simp_all only [Option.isSome_none, Bool.false_eq_true]
+lemma Part.eq_none_iff_forall_ne_some : o = Part.none ↔ ∀ a, o ≠ Part.some a := by
+  have := (@Part.ne_none_iff _ o).not
+  simp at this
+  exact this
+  -- cases o <;> simp
+lemma Part.not_none_iff_dom : (¬o=Part.none)↔(o.Dom) := by
+  apply Iff.intro
+  · intro a
+    simp [Part.eq_none_iff_forall_ne_some] at a
+    rcases a with ⟨h1,h2⟩
+    rw [h2]
+    exact trivial
+  · intro a
+    apply Aesop.BuiltinRules.not_intro
+    intro a_1
+    subst a_1
+    exact a
+lemma Part.ne_of_get_ne {p1 p2:Part ℕ} {h1:p1.Dom} {h2:p2.Dom} (h:p1.get h1≠p2.get h2) : (p1≠p2) := by aesop
+lemma Part.ne_of_get_ne' {p1:Part ℕ} {h1:p1.Dom} (h:p1.get h1≠x) : (p1≠Part.some x) := by aesop
 
-instance : IsRefl (ℕ → ℕ) TuringReducible where refl _ := .rfl
+-- variable {α:Type*} {β:Type*} {σ:Type*}
+-- variable [Primcodable α] [Primcodable β] [Primcodable σ]
 
-theorem TuringReducible.trans (hg : f ≤ᵀᶠ g) (hh : g ≤ᵀᶠ h) : f ≤ᵀᶠ h := by
-  generalize z : (↑f:ℕ→.ℕ)=x at hg
-  simp only [TuringReducible,z] at *
-  induction hg with
+-- @[simp] abbrev Nat.l (n:ℕ) := n.unpair.1
+-- @[simp] abbrev Nat.r (n:ℕ) := n.unpair.2
+def Nat.l (n:ℕ) := n.unpair.1
+def Nat.r (n:ℕ) := n.unpair.2
+@[simp] theorem pair_l : (Nat.pair x y).l = x := by simp [Nat.l]
+@[simp] theorem pair_r : (Nat.pair x y).r = y := by simp [Nat.r]
+@[simp] theorem pair_lr : (Nat.pair x.l x.r) = x := by simp [Nat.r, Nat.l]
+@[simp] theorem unpair1_to_l {n:ℕ} : (n.unpair.1) = n.l := by simp [Nat.l]
+@[simp] theorem unpair2_to_r {n:ℕ} : (n.unpair.2) = n.r := by simp [Nat.r]
+@[simp, reducible]
+def Nat.unpaired2 {α} (f : ℕ → ℕ → α) (n : ℕ) : α := f n.l n.r
+-- @[simp, reducible]
+-- def unpaired {α} (f : ℕ → ℕ → α) (n : ℕ) : α := f n.unpair.1 n.unpair.2
+@[simp] abbrev Nat.fzero:ℕ→ℕ:=λ_↦0
+
+def n2b (n:ℕ) : Bool := if n=0 then false else true
+def b2n (b:Bool) : ℕ := if b then 1 else 0
+def n2b' (n:ℕ) : Bool := if n=0 then true else false
+def b'2n (b:Bool) : ℕ := if b then 0 else 1
+open Denumerable
+open Encodable
+abbrev n2o := @ofNat (Option ℕ) _
+abbrev o2n := @encode (Option ℕ) _
+
+-- TODO: maybe delete the below?
+namespace Computability.Code.nc_to_nn
+@[coe] protected def lift (f:ℕ→Code) : ℕ→ℕ := fun x => c2n (f x)
+instance : Coe (ℕ→Code) (ℕ→ℕ) := ⟨Computability.Code.nc_to_nn.lift⟩
+end Computability.Code.nc_to_nn
+-- namespace Computability.Code.cn_to_nn
+-- @[coe] protected def lift (f:Code→ℕ) : ℕ→ℕ := fun x => (f x)
+-- instance coe : Coe (Code→ℕ) (ℕ→ℕ) := ⟨Computability.Code.cn_to_nn.lift⟩
+-- end Computability.Code.cn_to_nn
+namespace Computability.Code.cc_to_nn
+@[coe] protected def lift (f:Code→Code) : ℕ→ℕ := c2n ∘ f ∘ n2c
+instance : Coe (Code→Code) (ℕ→ℕ) := ⟨Computability.Code.cc_to_nn.lift⟩
+end Computability.Code.cc_to_nn
+
+-- conversions between oracle and non-oracle versions
+-- lemma PrimrecIn.PrimrecIn_Empty (h:Nat.PrimrecIn (λ _ ↦ 0) f):Nat.Primrec f := by
+--   induction' h with g hg g h _ _ ih₁ ih₂ g h _ _ ih₁ ih₂ g h _ _ ih₁ ih₂ g _ ih
+--   repeat {constructor}
+--   · (expose_names; exact Nat.Primrec.pair a_ih a_ih_1)
+--   repeat {constructor; assumption; try assumption}
+--   (expose_names; exact Nat.Primrec.prec a_ih a_ih_1)
+-- lemma PrimrecIn.PrimrecIn₂_Empty {f:α→β→σ} (h:PrimrecIn₂ (λ _ ↦ 0) f):Primrec₂ f := by
+--   unfold PrimrecIn₂ at h
+--   unfold Primrec₂
+--   apply PrimrecIn.PrimrecIn_Empty
+--   exact h
+-- theorem Primrec.to_PrimrecIn₂ {f:α→β→σ} (h:Primrec₂ f):PrimrecIn₂ O f := by
+--   unfold Primrec₂ at h
+--   unfold PrimrecIn₂
+--   apply Primrec.to_PrimrecIn
+--   exact h
+-- theorem PrimrecIn.PrimrecIn₂_iff_Primrec₂ {f:α→β→σ}:(∀O,PrimrecIn₂ O f) ↔ Primrec₂ f := by
+--   constructor
+--   · exact fun a ↦ PrimrecIn₂_Empty (a fun x ↦ 0)
+--   · exact fun a O ↦ Primrec.to_PrimrecIn₂ a
+-- theorem PrimrecIn.PrimrecIn_iff_Primrec:(∀O,Nat.PrimrecIn O f) ↔ Nat.Primrec f := by
+--   constructor
+--   · exact fun a ↦ PrimrecIn.PrimrecIn_Empty (a fun x ↦ 0)
+--   · exact fun a O ↦ Nat.Primrec.to_PrimrecIn a
+
+-- templates for primrec constructions as codes
+namespace Computability.Code
+@[aesop safe, cp] inductive code_prim:Code → Prop
+| zero:code_prim zero
+| succ:code_prim succ
+| left:code_prim left
+| right:code_prim right
+| oracle:code_prim oracle
+| pair {a b:Code} (ha:code_prim a) (hb:code_prim b):code_prim (pair a b)
+| comp {a b:Code} (ha:code_prim a) (hb:code_prim b):code_prim (comp a b)
+| prec {a b:Code} (ha:code_prim a) (hb:code_prim b):code_prim (prec a b)
+@[cp] theorem zero_ev_pr : code_prim zero := code_prim.zero
+@[cp] theorem succ_ev_pr : code_prim succ := code_prim.succ
+@[cp] theorem left_ev_pr : code_prim left := code_prim.left
+@[cp] theorem right_ev_pr : code_prim right := code_prim.right
+@[cp] theorem oracle_ev_pr : code_prim oracle := code_prim.oracle
+@[cp] theorem pair_ev_pr (ha:code_prim a) (hb:code_prim b) : code_prim (pair a b) := code_prim.pair ha hb
+@[cp] theorem comp_ev_pr (ha:code_prim a) (hb:code_prim b) : code_prim (comp a b) := code_prim.comp ha hb
+@[cp] theorem prec_ev_pr (ha:code_prim a) (hb:code_prim b) : code_prim (prec a b) := code_prim.prec ha hb
+def code_total (O) (c:Code) := ∀x, (eval O c x).Dom
+@[simp] theorem zero_total {O} : code_total O zero := λ _ ↦ trivial
+@[simp] theorem left_total {O} : code_total O left := λ _ ↦ trivial
+@[simp] theorem right_total {O} : code_total O right := λ _ ↦ trivial
+@[simp] theorem succ_total {O} : code_total O succ := λ _ ↦ trivial
+@[simp] theorem oracle_total {O} : code_total O oracle := λ _ ↦ trivial
+theorem total_pair_iff : (code_total O cf) ∧ (code_total O cg) ↔ (code_total O (pair cf cg)) :=
+  ⟨
+    λ h x ↦ ⟨h.left x, h.right x⟩
+  ,
+    λ h ↦ ⟨λ x ↦ Part.left_dom_of_sub_dom (h x) , λ x ↦ Part.right_dom_of_div_dom (h x)⟩
+  ⟩
+@[simp] theorem total_pair_of (hcf : code_total O cf) (hcg : code_total O cg) : (code_total O (pair cf cg)) := total_pair_iff.mp ⟨hcf,hcg⟩
+theorem total_comp_of (hcf : code_total O cf) (hcg : code_total O cg) : (code_total O (comp cf cg)) := by
+  intro x
+  simp [eval]
+  use hcg x
+  exact hcf ((eval O cg x).get (hcg x))
+@[simp] theorem total_of_pair_left {O} (h:code_total O (pair cf cg)) : code_total O cf :=
+  (total_pair_iff.mpr h).left
+@[simp] theorem total_of_pair_right {O} (h:code_total O (pair cf cg)) : code_total O cg :=
+  (total_pair_iff.mpr h).right
+@[simp] theorem total_of_comp_left {O} (h:code_total O (comp cf cg)) : code_total O cg := by
+  intro h2
+  exact Part.Dom.of_bind (h h2)
+@[simp] theorem total_of_comp_right {O} (h:code_total O (comp cf cg)) : ∀x, (eval O cf ((eval O cg x).get (Part.Dom.of_bind (h x)))).Dom := by
+  exact fun x ↦ Part.right_dom_of_div_dom (h x)
+@[simp] theorem total_of_prec_left {O} (h:code_total O (prec cf cg)) : code_total O cf := by
+  intro x
+  unfold code_total at h
+  simp [eval] at h
+  have hx := h (Nat.pair x 0)
+  simp at hx
+  exact hx
+-- @[simp] theorem total_of_prec_right {O} (h:code_total O (prec cf cg)) : code_total O cf := by
+--   intro x
+--   unfold code_total at h
+--   simp [eval] at h
+--   have hx := h (Nat.pair x 0)
+--   simp at hx
+--   exact hx
+
+  -- exact?
+  -- exact fun x ↦ Part.right_dom_of_div_dom (h x)
+
+theorem prim_total (h:code_prim c): code_total O c := by
+  unfold code_total
+  induction h with
+  | zero                   => simp [eval];
+  | succ                   => simp [eval];
+  | left                   => simp [eval];
+  | right                  => simp [eval];
+  | oracle                 => simp [eval];
+  | pair ha hb ha_ih hb_ih => simp [eval, Seq.seq]; exact fun x ↦ ⟨ha_ih x, hb_ih x⟩
+  | comp ha hb ha_ih hb_ih =>
+    simp [eval]
+    intro x
+    use hb_ih x
+    (expose_names; exact ha_ih ((eval O b x).get (hb_ih x)))
+  | prec ha hb ha_ih hb_ih =>
+    expose_names
+    simp [eval]
+    intro x
+    induction x.r with
+    | zero => exact ha_ih x.l
+    | succ y' IH' =>
+
+      simp
+      expose_names;
+      use IH'
+      apply hb_ih
+-- def eval_total (O:ℕ→ℕ) (c:Code) {h:code_total O c}:ℕ→ℕ := fun x => (eval O c x).get (h x)
+theorem eval_total_comp (h:code_total O (comp cf cg)) :
+  eval O (comp cf cg) x = Part.some ((eval O cf ((eval O cg x).get (Part.Dom.of_bind (h x)))).get (total_of_comp_right h x)) := by
+    simp
+    simp [eval]
+    exact Part.Dom.bind (Part.Dom.of_bind (h x)) (eval O cf)
+def evalt (O:ℕ→ℕ) (c:Code) (h:code_total O c) : ℕ→ℕ := λ x ↦ (eval O c x).get (h x)
+-- def eval_total (O:ℕ→ℕ) (c:Code) (h:code_total O c) : ℕ→ℕ := match c with
+-- | zero       => λ _ ↦ 0
+-- | succ       => Nat.succ
+-- | left       => Nat.l
+-- | right      => Nat.r
+-- | oracle     => O
+-- | pair cf cg => fun n => Nat.pair (eval_total O cf (total_of_pair_left h) n) (eval_total O cg (total_of_pair_right
+--   h) n)
+-- | comp cf cg => fun x => (eval O cf ((eval O cg x).get (Part.Dom.of_bind (h x)))).get (total_of_comp_right h x)
+-- | prec cf cg => fun x => (x.r).rec (eval_total O cf (total_of_prec_left h) x.l) fun y IH => (eval_total O cg (sorry)) <| Nat.pair x.l <| Nat.pair y IH
+-- | rfind' _ => 0
+noncomputable def Part.getD (p:Part ℕ) : ℕ := if h:p.Dom then p.get h else 0
+noncomputable def eval_total (O:ℕ→ℕ) (c:Code) : ℕ→ℕ := match c with
+| zero       => λ _ ↦ 0
+| succ       => Nat.succ
+| left       => Nat.l
+| right      => Nat.r
+| oracle     => O
+| pair cf cg => fun x => Nat.pair (eval_total O cf x) (eval_total O cg x)
+| comp cf cg => fun x => eval_total O cf (eval_total O cg x)
+| prec cf cg => unpaired fun z n => n.rec (eval_total O cf z) fun y IH => (eval_total O cg) <| Nat.pair z <| Nat.pair y IH
+| rfind' cf =>  Nat.unpaired fun a m => ((Nat.rfind fun n => (fun x => x = 0) <$> eval_total O cf (Nat.pair a (n + m))).map (· + m)).getD
+@[simp] def eval_prim (O:ℕ→ℕ):Code→ℕ→ℕ
+| zero       => λ _ ↦ 0
+| succ       => Nat.succ
+| left       => Nat.l
+| right      => Nat.r
+| oracle     => O
+| pair cf cg => fun x => Nat.pair (eval_prim O cf x) (eval_prim O cg x)
+| comp cf cg => fun x => eval_prim O cf (eval_prim O cg x)
+| prec cf cg => unpaired fun z n => n.rec (eval_prim O cf z) fun y IH => (eval_prim O cg) <| Nat.pair z <| Nat.pair y IH
+| rfind' _ => λ _ ↦ 0
+
+theorem eval_prim_eq_eval (h:code_prim c):eval_prim O c = eval O c := by
+  induction h with
+  | zero => exact rfl
+  | succ => exact rfl
+  | left => exact rfl
+  | right => exact rfl
+  | oracle => exact rfl
+  | pair ha hb ha_ih hb_ih =>
+    unfold eval_prim
+    simp [eval]
+    funext xs
+    simp [Seq.seq]
+    expose_names
+    simp only [show eval O a xs = Part.some (eval_prim O a xs) from by exact congrFun (_root_.id (Eq.symm ha_ih)) xs]
+    simp only [show eval O b xs = Part.some (eval_prim O b xs) from by exact congrFun (_root_.id (Eq.symm hb_ih)) xs]
+    simp
+  | comp ha hb ha_ih hb_ih =>
+    unfold eval_prim
+    simp [eval]
+    funext xs
+    simp
+    expose_names
+    simp only [show eval O b xs = Part.some (eval_prim O b xs) from by exact congrFun (_root_.id (Eq.symm hb_ih)) xs]
+    simp
+    simp only [show eval O a (eval_prim O b xs) = Part.some (eval_prim O a (eval_prim O b xs)) from by exact congrFun (_root_.id (Eq.symm ha_ih)) (eval_prim O b xs)]
+  | prec ha hb ha_ih hb_ih =>
+    unfold eval_prim
+    simp [eval]
+    funext xs
+    simp
+    expose_names
+    induction xs.r with
+    | zero =>
+      simp
+      simp only [show eval O a xs.l = Part.some (eval_prim O a xs.l) from by exact congrFun (_root_.id (Eq.symm ha_ih)) xs.l]
+    | succ y' IH' =>
+      have h0:@Nat.rec (fun x ↦ Part ℕ) (eval O a xs.l) (fun y IH ↦ IH.bind fun i ↦ eval O b (Nat.pair xs.l (Nat.pair y i))) (y'+1) = ((@Nat.rec (fun x ↦ Part ℕ) (eval O a xs.l)
+  (fun y IH ↦ IH.bind fun i ↦ eval O b (Nat.pair xs.l (Nat.pair y i))) y').bind fun i ↦ eval O b (Nat.pair xs.l (Nat.pair y' i))) := by
+        exact rfl
+      rw [h0]
+      rw [←IH']
+      rw [Part.bind_some]
+      simp
+      rw [show eval O b ((Nat.pair xs.l (Nat.pair y' (Nat.rec (eval_prim O a xs.l) (fun y IH ↦ eval_prim O b (Nat.pair xs.l (Nat.pair y IH))) y')))) = Part.some (eval_prim O b ((Nat.pair xs.l (Nat.pair y' (Nat.rec (eval_prim O a xs.l) (fun y IH ↦ eval_prim O b (Nat.pair xs.l (Nat.pair y IH))) y'))))) from by exact congrFun (_root_.id (Eq.symm hb_ih)) ((Nat.pair xs.l (Nat.pair y' (Nat.rec (eval_prim O a xs.l) (fun y IH ↦ eval_prim O b (Nat.pair xs.l (Nat.pair y IH))) y'))))]
+theorem eval_prim_eq_eval_ext (h:code_prim c): eval O c x = eval_prim O c x := congrFun (_root_.id (Eq.symm (@eval_prim_eq_eval c O h))) x
+-- theorem eval_total_eq_eval (h:code_total O c):eval_total O c = eval O c := by
+--   sorry
+  -- induction c generalizing h with
+  -- | zero => exact rfl
+  -- | succ => exact rfl
+  -- | left => exact rfl
+  -- | right => exact rfl
+  -- | oracle => exact rfl
+  -- | pair ha hb ha_ih hb_ih =>
+  --   unfold eval
+  --   rw [← ha_ih (total_of_pair_left h)]
+  --   rw [← hb_ih (total_of_pair_right h)]
+  --   exact pair' (eval_total O ha) (eval_total O hb)
+  -- | comp ha hb ha_ih hb_ih =>
+  --   unfold eval_total
+  --   simp [eval]
+  --   funext xs
+  --   simp
+  --   expose_names
+  --   simp only [show eval O b xs = Part.some (eval_total O b xs) from by exact congrFun (_root_.id (Eq.symm hb_ih)) xs]
+  --   simp
+  --   simp only [show eval O a (eval_total O b xs) = Part.some (eval_total O a (eval_total O b xs)) from by exact congrFun (_root_.id (Eq.symm ha_ih)) (eval_total O b xs)]
+  -- | prec ha hb ha_ih hb_ih =>
+  --   unfold eval
+  --   unfold eval_total
+  --   have := ha_ih ?_
+  --   rotate_left
+  --   exact total_of_prec_left h
+  --   rw [← this]
+
+  --   simp
+  --   funext xs
+  --   simp
+
+  --   induction xs.r with
+  --   | zero => simp
+  --   | succ n ih =>
+  --     simp
+  --     rw [← ih]
+  --     simp [Part.bind_some]
+
+  --     sorry
+
+  --   have := hb_ih ?_
+  --   rotate_left
+
+  -- | rfind' cf hcf =>
+  --   sorry
+@[simp 1000] theorem RecursiveIn_of_eval : Nat.RecursiveIn O (eval O c) := by
+  induction c with
   | zero => exact Nat.RecursiveIn.zero
   | succ => exact Nat.RecursiveIn.succ
   | left => exact Nat.RecursiveIn.left
   | right => exact Nat.RecursiveIn.right
-  | oracle => exact hh
-  | pair hf hh hf_ih hh_ih => (expose_names; exact Nat.RecursiveIn.pair hf_ih hh_ih)
-  | comp hf hh hf_ih hh_ih => (expose_names; exact Nat.RecursiveIn.comp hf_ih hh_ih)
-  | prec hf hh hf_ih hh_ih => (expose_names; exact Nat.RecursiveIn.prec hf_ih hh_ih)
-  | rfind hf ih => (expose_names; exact Nat.RecursiveIn.rfind ih)
+  | oracle => exact Nat.RecursiveIn.oracle
+  | pair ha hb ha_ih hb_ih => unfold eval; exact Nat.RecursiveIn.pair (ha_ih) (hb_ih)
+  | comp ha hb ha_ih hb_ih => unfold eval; exact Nat.RecursiveIn.comp (ha_ih) (hb_ih)
+  | prec ha hb ha_ih hb_ih => unfold eval; exact Nat.RecursiveIn.prec (ha_ih) (hb_ih)
+  | rfind' ha ha_ih => unfold eval; exact RecursiveIn.rfind ha_ih
+@[simp 1000] theorem code_prim_prop : Nat.PrimrecIn O (eval_prim O c) := by
+  induction c with
+  | zero => exact Nat.PrimrecIn.zero
+  | succ => exact Nat.PrimrecIn.succ
+  | left => exact Nat.PrimrecIn.left
+  | right => exact Nat.PrimrecIn.right
+  | oracle => exact Nat.PrimrecIn.oracle
+  | pair ha hb ha_ih hb_ih => unfold eval_prim; exact Nat.PrimrecIn.pair (ha_ih) (hb_ih)
+  | comp ha hb ha_ih hb_ih => unfold eval_prim; exact Nat.PrimrecIn.comp (ha_ih) (hb_ih)
+  | prec ha hb ha_ih hb_ih => unfold eval_prim; exact Nat.PrimrecIn.prec (ha_ih) (hb_ih)
+  | rfind' ha ha_ih => exact Nat.PrimrecIn.zero
+theorem code_prim_of_primrecIn (h:Nat.PrimrecIn O f) : ∃ c, code_prim c ∧ f=eval_prim O c := by
+  induction h with
+  | zero => use Code.zero; exact ⟨code_prim.zero,rfl⟩
+  | succ => use Code.succ; exact ⟨code_prim.succ,rfl⟩
+  | left => use Code.left; exact ⟨code_prim.left,rfl⟩
+  | right => use Code.right; exact ⟨code_prim.right,rfl⟩
+  | oracle => use Code.oracle; exact ⟨code_prim.oracle,rfl⟩
+  | pair pf pg ef eg =>
+    rcases ef with ⟨cf,hcf⟩
+    rcases eg with ⟨cg,hcg⟩
+    use Code.pair cf cg;
+    constructor
+    · exact code_prim.pair hcf.left hcg.left
+    · simp only [eval_prim]; rw [hcf.right, hcg.right]
+  | comp pf pg ef eg =>
+    rcases ef with ⟨cf,hcf⟩
+    rcases eg with ⟨cg,hcg⟩
+    use Code.comp cf cg;
+    constructor
+    · exact code_prim.comp hcf.left hcg.left
+    · simp only [eval_prim]; rw [hcf.right, hcg.right]
+  | prec pf pg ef eg =>
+    rcases ef with ⟨cf,hcf⟩
+    rcases eg with ⟨cg,hcg⟩
+    use Code.prec cf cg;
+    constructor
+    · exact code_prim.prec hcf.left hcg.left
+    · simp only [eval_prim]; rw [hcf.right, hcg.right]
 
-theorem TuringReducible.trans' (hg : Nat.RecursiveIn g f) (hh : g ≤ᵀᶠ h) : Nat.RecursiveIn h f := by
-  generalize z : (↑f:ℕ→.ℕ)=x at hg
-  simp only [TuringReducible,z] at *
-  induction hg with
-  | zero => exact Nat.RecursiveIn.zero
-  | succ => exact Nat.RecursiveIn.succ
-  | left => exact Nat.RecursiveIn.left
-  | right => exact Nat.RecursiveIn.right
-  | oracle => exact hh
-  | pair hf hh hf_ih hh_ih => (expose_names; exact Nat.RecursiveIn.pair hf_ih hh_ih)
-  | comp hf hh hf_ih hh_ih => (expose_names; exact Nat.RecursiveIn.comp hf_ih hh_ih)
-  | prec hf hh hf_ih hh_ih => (expose_names; exact Nat.RecursiveIn.prec hf_ih hh_ih)
-  | rfind hf ih => (expose_names; exact Nat.RecursiveIn.rfind ih)
-
-instance : IsTrans (ℕ→ℕ) TuringReducible := ⟨@TuringReducible.trans⟩
-instance : IsPreorder (ℕ→ℕ) TuringReducible where refl := .refl
-theorem TuringEquivalent.equivalence : Equivalence TuringEquivalent := (AntisymmRel.setoid _ _).iseqv
-@[refl] protected theorem TuringEquivalent.refl (f : ℕ→ℕ) : f ≡ᵀᶠ f := Equivalence.refl equivalence f
-@[symm] theorem TuringEquivalent.symm {f g : ℕ→ℕ} (h : f ≡ᵀᶠ g) : g ≡ᵀᶠ f := Equivalence.symm equivalence h
-@[trans] theorem TuringEquivalent.trans {f g h : ℕ→ℕ} (h₁ : f ≡ᵀᶠ g) (h₂ : g ≡ᵀᶠ h) : f ≡ᵀᶠ h := Equivalence.trans equivalence h₁ h₂
-
-/--
-Instance declaring that `Nat.RecursiveIn` is a preorder.
--/
-instance : IsPreorder (ℕ→ℕ) TuringReducible where
-  refl := TuringReducible.refl
-  trans := @TuringReducible.trans
-
-abbrev FuncTuringDegree :=
-  Antisymmetrization _ TuringReducible
-private instance : Preorder (ℕ→ℕ) where
-  le := TuringReducible
-  le_refl := .refl
-  le_trans _ _ _ := TuringReducible.trans
-  lt := TuringReducibleStrict
-
-
-
--- helper funcs:
-
--- @[simp] lemma Nat.RecursiveIn.partCompTotal {O:ℕ→ℕ} {f:ℕ→.ℕ} {g:ℕ→ℕ} (h1: Nat.RecursiveIn O f) (h2: Nat.RecursiveIn O g):(Nat.RecursiveIn O ↑(f∘g)) := by
---   have h3:(↑(f∘g):ℕ→.ℕ) = fun x => g x >>= (↑f:ℕ→.ℕ) := by
---     funext xs
---     simp only [Function.comp_apply, Part.coe_some, Part.bind_eq_bind, Part.bind_some]
---   rw [h3]
---   exact comp h1 h2
--- @[simp] lemma Nat.RecursiveIn.totalComp {O:ℕ→ℕ} {f g:ℕ→ℕ} (h1: Nat.RecursiveIn O f) (h2: Nat.RecursiveIn O g):(Nat.RecursiveIn O ↑(f∘g)) := by
---   have h3:(↑(f∘g):ℕ→.ℕ) = fun x => g x >>= (↑f:ℕ→.ℕ) := by
---     funext xs
---     simp only [PFun.coe_val, Function.comp_apply, Part.coe_some, Part.bind_eq_bind, Part.bind_some]
---   rw [h3]
---   exact comp h1 h2
--- @[simp] lemma Nat.RecursiveIn.id {O:ℕ→ℕ}:Nat.RecursiveIn O fun x => x := by apply of_primrec Nat.Primrec.id
--- @[simp] lemma Nat.RecursiveIn.someTotal (O:ℕ→ℕ) (f:ℕ→ℕ) (h1: Nat.RecursiveIn O f): Nat.RecursiveIn O fun x => Part.some (f x) := by
---   apply Nat.RecursiveIn.totalComp
---   · exact h1
---   · apply Nat.RecursiveIn.id
--- @[simp] lemma Nat.RecursiveIn.pair' (f g:ℕ→ℕ):((↑fun x ↦ Nat.pair (f x) (g x)):ℕ→.ℕ)= fun (x:ℕ) => (Nat.pair <$> (f x) <*> (g x)) := by
---   simp [Seq.seq]
---   funext xs
---   simp only [PFun.coe_val]
--- @[simp] lemma Nat.RecursiveIn.totalComp' {O:ℕ→ℕ} {f g:ℕ→ℕ} (hf: Nat.RecursiveIn O f) (hg: Nat.RecursiveIn O g): (Nat.RecursiveIn O (fun x => (f (g x)):ℕ→ℕ) ) := by apply Nat.RecursiveIn.totalComp (hf) (hg)
--- @[simp] lemma Nat.RecursiveIn.comp₂ {O:ℕ→ℕ} {f:ℕ→ℕ→.ℕ} {g h:ℕ→ℕ} (hf: Nat.RecursiveIn O fun x => f x.unpair.1 x.unpair.2) (hg: Nat.RecursiveIn O g) (hh: Nat.RecursiveIn O h): (Nat.RecursiveIn O (fun x => (f (g x) (h x))) ) := by
---   have main:(fun x => (f (g x) (h x))) = ((fun x => f x.unpair.1 x.unpair.2) ∘ (fun n ↦ Nat.pair (g n) (h n))) := by
---     funext xs
---     simp only [Function.comp_apply, unpair_pair]
---   rw [main]
---   refine partCompTotal hf ?_
---   · rw [Nat.RecursiveIn.pair']
---     apply Nat.RecursiveIn.pair hg hh
--- @[simp] lemma Nat.RecursiveIn.totalComp₂ {O:ℕ→ℕ} {f:ℕ→ℕ→ℕ} {g h:ℕ→ℕ} (hf: Nat.RecursiveIn O fun x => f x.unpair.1 x.unpair.2) (hg: Nat.RecursiveIn O g) (hh: Nat.RecursiveIn O h): (Nat.RecursiveIn O (fun x => (f (g x) (h x)):ℕ→ℕ) ) := by
---   have main:(fun x => (f (g x) (h x)):ℕ→ℕ) = ((fun x => f x.unpair.1 x.unpair.2) ∘ (fun n ↦ Nat.pair (g n) (h n))) := by
---     funext xs
---     simp only [Function.comp_apply, Nat.unpair_pair]
---   rw [main]
---   apply Nat.RecursiveIn.totalComp
---   · exact hf
---   · rw [Nat.RecursiveIn.pair']
---     apply Nat.RecursiveIn.pair hg hh
-
--- @[simp] lemma Nat.PrimrecIn.totalComp {O:ℕ→ℕ} {f g:ℕ→ℕ} (h1: Nat.PrimrecIn O f) (h2: Nat.PrimrecIn O g):(Nat.PrimrecIn O ↑(f∘g)) := by
---   rw [show (f∘g) = fun x => f (g x) from rfl]
---   exact comp h1 h2
--- @[simp] lemma Nat.PrimrecIn.comp₂ {O:ℕ→ℕ} {f:ℕ→ℕ→ℕ} {g h:ℕ→ℕ} (hf: Nat.PrimrecIn O fun x => f x.unpair.1 x.unpair.2) (hg: Nat.PrimrecIn O g) (hh: Nat.PrimrecIn O h): (Nat.PrimrecIn O (fun x => (f (g x) (h x)):ℕ→ℕ) ) := by
---   have main:(fun x => (f (g x) (h x)):ℕ→ℕ) = ((fun x => f x.unpair.1 x.unpair.2) ∘ (fun n ↦ Nat.pair (g n) (h n))) := by
---     funext xs
---     simp only [Function.comp_apply, Nat.unpair_pair]
---   rw [main]
---   apply Nat.PrimrecIn.totalComp
---   · exact hf
---   · apply Nat.PrimrecIn.pair hg hh
+end Computability.Code
