Computability/Order.lean
@@ -1,0 +1,123 @@
+import Computability.Oracle
+import Mathlib.Order.Antisymmetrization
+
+@[simp] abbrev TuringReducible (f g : ℕ → ℕ) : Prop := Nat.RecursiveIn g f
+@[simp] abbrev TuringReducibleStrict (f g : ℕ → ℕ) : Prop := Nat.RecursiveIn g f ∧ ¬ Nat.RecursiveIn f g
+@[simp] abbrev TuringEquivalent (f g : ℕ → ℕ) : Prop := AntisymmRel TuringReducible f g
+
+@[reducible,simp,inherit_doc] scoped[Computability] infix:50 " ≤ᵀᶠ " => TuringReducible
+@[reducible,simp,inherit_doc] scoped[Computability] infix:50 " ≡ᵀᶠ " => TuringEquivalent
+@[reducible,simp,inherit_doc] scoped[Computability] infix:50 " <ᵀᶠ " => TuringReducibleStrict
+
+open scoped Computability
+
+protected theorem TuringReducible.refl (f : ℕ → ℕ) : f ≤ᵀᶠ f := by exact Nat.RecursiveIn.oracle
+protected theorem TuringReducible.rfl : f ≤ᵀᶠ f := .refl _
+
+instance : IsRefl (ℕ → ℕ) TuringReducible where refl _ := .rfl
+
+theorem TuringReducible.trans (hg : f ≤ᵀᶠ g) (hh : g ≤ᵀᶠ h) : f ≤ᵀᶠ h := by
+  generalize z : (↑f:ℕ→.ℕ)=x at hg
+  simp only [TuringReducible,z] at *
+  induction hg with
+  | zero => exact Nat.RecursiveIn.zero
+  | succ => exact Nat.RecursiveIn.succ
+  | left => exact Nat.RecursiveIn.left
+  | right => exact Nat.RecursiveIn.right
+  | oracle => exact hh
+  | pair hf hh hf_ih hh_ih => (expose_names; exact Nat.RecursiveIn.pair hf_ih hh_ih)
+  | comp hf hh hf_ih hh_ih => (expose_names; exact Nat.RecursiveIn.comp hf_ih hh_ih)
+  | prec hf hh hf_ih hh_ih => (expose_names; exact Nat.RecursiveIn.prec hf_ih hh_ih)
+  | rfind hf ih => (expose_names; exact Nat.RecursiveIn.rfind ih)
+
+theorem TuringReducible.trans' (hg : Nat.RecursiveIn g f) (hh : g ≤ᵀᶠ h) : Nat.RecursiveIn h f := by
+  generalize z : (↑f:ℕ→.ℕ)=x at hg
+  simp only [TuringReducible,z] at *
+  induction hg with
+  | zero => exact Nat.RecursiveIn.zero
+  | succ => exact Nat.RecursiveIn.succ
+  | left => exact Nat.RecursiveIn.left
+  | right => exact Nat.RecursiveIn.right
+  | oracle => exact hh
+  | pair hf hh hf_ih hh_ih => (expose_names; exact Nat.RecursiveIn.pair hf_ih hh_ih)
+  | comp hf hh hf_ih hh_ih => (expose_names; exact Nat.RecursiveIn.comp hf_ih hh_ih)
+  | prec hf hh hf_ih hh_ih => (expose_names; exact Nat.RecursiveIn.prec hf_ih hh_ih)
+  | rfind hf ih => (expose_names; exact Nat.RecursiveIn.rfind ih)
+
+instance : IsTrans (ℕ→ℕ) TuringReducible := ⟨@TuringReducible.trans⟩
+instance : IsPreorder (ℕ→ℕ) TuringReducible where refl := .refl
+theorem TuringEquivalent.equivalence : Equivalence TuringEquivalent := (AntisymmRel.setoid _ _).iseqv
+@[refl] protected theorem TuringEquivalent.refl (f : ℕ→ℕ) : f ≡ᵀᶠ f := Equivalence.refl equivalence f
+@[symm] theorem TuringEquivalent.symm {f g : ℕ→ℕ} (h : f ≡ᵀᶠ g) : g ≡ᵀᶠ f := Equivalence.symm equivalence h
+@[trans] theorem TuringEquivalent.trans {f g h : ℕ→ℕ} (h₁ : f ≡ᵀᶠ g) (h₂ : g ≡ᵀᶠ h) : f ≡ᵀᶠ h := Equivalence.trans equivalence h₁ h₂
+
+/--
+Instance declaring that `Nat.RecursiveIn` is a preorder.
+-/
+instance : IsPreorder (ℕ→ℕ) TuringReducible where
+  refl := TuringReducible.refl
+  trans := @TuringReducible.trans
+
+abbrev FuncTuringDegree :=
+  Antisymmetrization _ TuringReducible
+private instance : Preorder (ℕ→ℕ) where
+  le := TuringReducible
+  le_refl := .refl
+  le_trans _ _ _ := TuringReducible.trans
+  lt := TuringReducibleStrict
+
+
+
+-- helper funcs:
+
+-- @[simp] lemma Nat.RecursiveIn.partCompTotal {O:ℕ→ℕ} {f:ℕ→.ℕ} {g:ℕ→ℕ} (h1: Nat.RecursiveIn O f) (h2: Nat.RecursiveIn O g):(Nat.RecursiveIn O ↑(f∘g)) := by
+--   have h3:(↑(f∘g):ℕ→.ℕ) = fun x => g x >>= (↑f:ℕ→.ℕ) := by
+--     funext xs
+--     simp only [Function.comp_apply, Part.coe_some, Part.bind_eq_bind, Part.bind_some]
+--   rw [h3]
+--   exact comp h1 h2
+-- @[simp] lemma Nat.RecursiveIn.totalComp {O:ℕ→ℕ} {f g:ℕ→ℕ} (h1: Nat.RecursiveIn O f) (h2: Nat.RecursiveIn O g):(Nat.RecursiveIn O ↑(f∘g)) := by
+--   have h3:(↑(f∘g):ℕ→.ℕ) = fun x => g x >>= (↑f:ℕ→.ℕ) := by
+--     funext xs
+--     simp only [PFun.coe_val, Function.comp_apply, Part.coe_some, Part.bind_eq_bind, Part.bind_some]
+--   rw [h3]
+--   exact comp h1 h2
+-- @[simp] lemma Nat.RecursiveIn.id {O:ℕ→ℕ}:Nat.RecursiveIn O fun x => x := by apply of_primrec Nat.Primrec.id
+-- @[simp] lemma Nat.RecursiveIn.someTotal (O:ℕ→ℕ) (f:ℕ→ℕ) (h1: Nat.RecursiveIn O f): Nat.RecursiveIn O fun x => Part.some (f x) := by
+--   apply Nat.RecursiveIn.totalComp
+--   · exact h1
+--   · apply Nat.RecursiveIn.id
+-- @[simp] lemma Nat.RecursiveIn.pair' (f g:ℕ→ℕ):((↑fun x ↦ Nat.pair (f x) (g x)):ℕ→.ℕ)= fun (x:ℕ) => (Nat.pair <$> (f x) <*> (g x)) := by
+--   simp [Seq.seq]
+--   funext xs
+--   simp only [PFun.coe_val]
+-- @[simp] lemma Nat.RecursiveIn.totalComp' {O:ℕ→ℕ} {f g:ℕ→ℕ} (hf: Nat.RecursiveIn O f) (hg: Nat.RecursiveIn O g): (Nat.RecursiveIn O (fun x => (f (g x)):ℕ→ℕ) ) := by apply Nat.RecursiveIn.totalComp (hf) (hg)
+-- @[simp] lemma Nat.RecursiveIn.comp₂ {O:ℕ→ℕ} {f:ℕ→ℕ→.ℕ} {g h:ℕ→ℕ} (hf: Nat.RecursiveIn O fun x => f x.unpair.1 x.unpair.2) (hg: Nat.RecursiveIn O g) (hh: Nat.RecursiveIn O h): (Nat.RecursiveIn O (fun x => (f (g x) (h x))) ) := by
+--   have main:(fun x => (f (g x) (h x))) = ((fun x => f x.unpair.1 x.unpair.2) ∘ (fun n ↦ Nat.pair (g n) (h n))) := by
+--     funext xs
+--     simp only [Function.comp_apply, unpair_pair]
+--   rw [main]
+--   refine partCompTotal hf ?_
+--   · rw [Nat.RecursiveIn.pair']
+--     apply Nat.RecursiveIn.pair hg hh
+-- @[simp] lemma Nat.RecursiveIn.totalComp₂ {O:ℕ→ℕ} {f:ℕ→ℕ→ℕ} {g h:ℕ→ℕ} (hf: Nat.RecursiveIn O fun x => f x.unpair.1 x.unpair.2) (hg: Nat.RecursiveIn O g) (hh: Nat.RecursiveIn O h): (Nat.RecursiveIn O (fun x => (f (g x) (h x)):ℕ→ℕ) ) := by
+--   have main:(fun x => (f (g x) (h x)):ℕ→ℕ) = ((fun x => f x.unpair.1 x.unpair.2) ∘ (fun n ↦ Nat.pair (g n) (h n))) := by
+--     funext xs
+--     simp only [Function.comp_apply, Nat.unpair_pair]
+--   rw [main]
+--   apply Nat.RecursiveIn.totalComp
+--   · exact hf
+--   · rw [Nat.RecursiveIn.pair']
+--     apply Nat.RecursiveIn.pair hg hh
+
+-- @[simp] lemma Nat.PrimrecIn.totalComp {O:ℕ→ℕ} {f g:ℕ→ℕ} (h1: Nat.PrimrecIn O f) (h2: Nat.PrimrecIn O g):(Nat.PrimrecIn O ↑(f∘g)) := by
+--   rw [show (f∘g) = fun x => f (g x) from rfl]
+--   exact comp h1 h2
+-- @[simp] lemma Nat.PrimrecIn.comp₂ {O:ℕ→ℕ} {f:ℕ→ℕ→ℕ} {g h:ℕ→ℕ} (hf: Nat.PrimrecIn O fun x => f x.unpair.1 x.unpair.2) (hg: Nat.PrimrecIn O g) (hh: Nat.PrimrecIn O h): (Nat.PrimrecIn O (fun x => (f (g x) (h x)):ℕ→ℕ) ) := by
+--   have main:(fun x => (f (g x) (h x)):ℕ→ℕ) = ((fun x => f x.unpair.1 x.unpair.2) ∘ (fun n ↦ Nat.pair (g n) (h n))) := by
+--     funext xs
+--     simp only [Function.comp_apply, Nat.unpair_pair]
+--   rw [main]
+--   apply Nat.PrimrecIn.totalComp
+--   · exact hf
+--   · apply Nat.PrimrecIn.pair hg hh
