Computability/Use.lean
@@ -1,4 +1,4 @@
-import Computability.RecursiveInTheorems
+import Computability.Basic
 import Mathlib.Tactic.Linarith
 
 open List Nat
